src/program_proof/txn/twophase_refinement_defs.v
@@ -19,6 +19,7 @@ Existing Instances jrnl_spec_ext jrnl_spec_ffi_model jrnl_spec_ext_semantics jrn
 Section refinement_defs.
 Context `{!heapGS Σ}.
 Context `{!refinement_heapG Σ}.
+Context (JRNL_SIZE: nat).
 
 Existing Instance jrnlG0.
 
@@ -43,7 +44,8 @@ Definition twophase_names := unit.
 Definition twophase_get_names (Σ: gFunctors) (hG: twophaseG Σ) := tt.
 Definition twophase_update (Σ: gFunctors) (hG: twophaseG Σ) (n: twophase_names) := hG.
 
-Definition LVL_INIT : nat := 150.
+
+Definition LVL_INIT : nat := 1 + JRNL_SIZE.
 Definition LVL_INV : nat := 125.
 Definition LVL_OPS : nat := 100.
 
@@ -96,7 +98,9 @@ Definition twophase_crash_tok {Σ: gFunctors} {hG: heapGS Σ} {rG: refinement_he
 Definition twophase_init {Σ: gFunctors} {hG: heapGS Σ} {rG: refinement_heapG Σ} {aG : twophaseG Σ} : iProp Σ
   := (∃ γ dinit logm mt, twophase_crash_cond_full γ dinit logm mt ∗
           auth_map.map_ctx jrnlG_crash_toks_name 1 ((λ _, tt) <$> (bufObj_to_obj <$> mt)) ∗
-          jrnl_full_crash_tok ∗ jrnl_closed_frag).
+          jrnl_full_crash_tok ∗ jrnl_closed_frag ∗
+          pre_borrow ∗
+          ([∗ map] _ ↦ _ ∈ mt, pre_borrow)).
 
 Definition twophaseN : coPset := (∅ : coPset).
 
@@ -111,7 +115,7 @@ Definition twophase_val_interp {Σ: gFunctors} {hG: heapGS Σ} {rG: refinement_h
   end.
 
 Instance twophaseTy_model : specTy_model jrnl_ty.
-Proof.
+Proof using JRNL_SIZE.
  refine
   {| styG := twophaseG;
      sty_names := twophase_names;
