src/goose_lang/recovery_adequacy.v
@@ -5,12 +5,13 @@ From Perennial.algebra Require Import proph_map.
 From Perennial.goose_lang Require Import proofmode notation.
 From Perennial.program_logic Require Import recovery_weakestpre recovery_adequacy.
 From Perennial.goose_lang Require Export wpr_lifting.
-From Perennial.goose_lang Require Import typing adequacy lang.
+From Perennial.goose_lang Require Import typing adequacy lang crash_borrow.
 Set Default Proof Using "Type".
 
-Theorem heap_recv_adequacy `{ffi_sem: ffi_semantics} `{!ffi_interp ffi} {Hffi_adequacy:ffi_interp_adequacy} Σ `{hPre: !heapGpreS Σ} s k e r σ g φ φr φinv Φinv (HINITG: ffi_initgP g) (HINIT: ffi_initP σ.(world) g) :
+Theorem heap_recv_adequacy `{ffi_sem: ffi_semantics} `{!ffi_interp ffi} {Hffi_adequacy:ffi_interp_adequacy} Σ `{hPre: !heapGpreS Σ} s k e r σ g φ φr φinv Φinv (HINITG: ffi_initgP g) (HINIT: ffi_initP σ.(world) g) n :
   (∀ `{Hheap : !heapGS Σ},
-     ⊢ (ffi_local_start (heapG_ffiG) σ.(world) g -∗ trace_frag σ.(trace) -∗ oracle_frag σ.(oracle) ={⊤}=∗
+     ⊢ (ffi_local_start (heapG_ffiG) σ.(world) g -∗ trace_frag σ.(trace) -∗ oracle_frag σ.(oracle) -∗
+        pre_borrowN n ={⊤}=∗
        □ (∀ σ nt, state_interp σ nt -∗ |NC={⊤, ∅}=> ⌜ φinv σ ⌝) ∗
        □ (∀ hG (Hpf: @heapG_invG _ _ _ _ Hheap = @heapG_invG _ _ _ _ hG),
                      Φinv hG -∗ □ ∀ σ nt, state_interp σ nt -∗ |NC={⊤, ∅}=> ⌜ φinv σ ⌝) ∗
@@ -18,15 +19,16 @@ Theorem heap_recv_adequacy `{ffi_sem: ffi_semantics} `{!ffi_interp ffi} {Hffi_ad
   recv_adequate (CS := goose_crash_lang) s e r σ g (λ v _ _, φ v) (λ v _ _, φr v) (λ σ _, φinv σ).
 Proof.
   intros Hwp.
-  eapply (wp_recv_adequacy_inv _ _ _ heap_local_namesO crash_borrow_ginv_number _ _ _ _ _ _ _ _
-           (* (λ names0 Hinv Hc names, ∃ namesg, Φinv (heap_update_local _
-                                         (heap_update_pre _ _ Hinv Hc (heap_extend_local_names (@pbundleT _ _ names) namesg)) Hinv Hc (@pbundleT _ _ names)))%I *) _).
+  eapply (wp_recv_adequacy_inv _ _ _ heap_local_namesO (n * 4 + crash_borrow_ginv_number) _ _ _ _ _ _ _ _ _).
   iIntros (???) "".
   iMod (na_heap_name_init tls σ.(heap)) as (name_na_heap) "Hh".
   iMod (ffi_name_global_init _ _ g) as (ffi_namesg) "(Hgw&_)"; first auto.
   iMod (ffi_name_init _ _ σ.(world) g with "Hgw") as (ffi_names) "(Hw&Hgw&Hstart)"; first auto.
   iMod (trace_name_init σ.(trace) σ.(oracle)) as (name_trace) "(Htr&Htrfrag&Hor&Hofrag)".
-  iMod (credit_name_init crash_borrow_ginv_number) as (name_credit) "(Hcred_auth&Hcred&Htok)".
+  iMod (credit_name_init (n*4 + crash_borrow_ginv_number)) as (name_credit) "(Hcred_auth&Hcred&Htok)".
+  iDestruct (cred_frag_split with "Hcred") as "(Hpre&Hcred)".
+
+
   iAssert (|={⊤}=> crash_borrow_ginv)%I with "[Hcred]" as ">#Hinv".
   { rewrite /crash_borrow_ginv. iApply (inv_alloc _). iNext. eauto. }
   set (hnames := {| heap_heap_names := name_na_heap;
@@ -36,6 +38,7 @@ Proof.
                       heap_credit_names := name_credit
                  |}).
   set (hG := heap_update_pre _ hPre Hinv Hc hnames).
+  iDestruct (@cred_frag_to_pre_borrowN _ _ _ _ _ hG n with "Hpre") as "Hpre".
   iExists ({| pbundleT := heap_get_local_names Σ hG |}).
   iExists
     (λ t σ nt, let _ := heap_update_local Σ hG Hinv Hc (@pbundleT _ _ t) in
@@ -53,7 +56,7 @@ Proof.
   iExists _.
   iExists _.
   iExists ((λ names0 Hinv Hc names, Φinv (heap_update_local _ hG Hinv Hc (@pbundleT _ _ names)))).
-  iMod (Hwp hG with "[$] [$] [$]") as "(#H1&#H2&Hwp)".
+  iMod (Hwp hG with "[$] [$] [$] [$]") as "(#H1&#H2&Hwp)".
   iModIntro.
   iSplitR.
   { iModIntro. iIntros (??) "Hσ".
